Implement logarithmic argmax

code/experimental/he/hestarhs/src/Argmax.hs
@@ -6,6 +6,7 @@ import Universum
 
 import Control.Concurrent (threadDelay, withMVar)
 import Control.Concurrent.Async (concurrently)
+import Data.Array.IO
 import Data.Bits (testBit)
 import qualified Data.ByteString as BS
 import Data.List (findIndex, (!!))
@@ -21,6 +22,7 @@ import System.ZMQ4
 import Hacl
 import qualified Lib as L
 import Playground
+import TestHacl
 
 getCurrentTimeMs :: IO Integer
 getCurrentTimeMs = floor . (*1000) <$> getPOSIXTime
@@ -31,21 +33,33 @@ lMVar = unsafePerformIO $ newMVar ()
 log :: MonadIO m => Text -> m ()
 log x = do
     t <- liftIO getCurrentTimeMs
-    liftIO $ withMVar lMVar $ \() -> putTextLn (show t <> " " <> x) >> pure ()
+    liftIO $ withMVar lMVar $ \() ->
+      putTextLn (show (t`div`1000) <> "." <> show (t`mod`1000) <> " " <> x) >> pure ()
 
+lambda :: Integral a => a
+lambda = 80
+
+-- taken from https://wiki.haskell.org/Random_shuffle
 shuffle :: [a] -> IO [a]
-shuffle [] = pure []
 shuffle xs = do
-    let l = length xs
-    let accum used current j = if j == l then pure current else do
-          ix <- randomRIO (0,l-1) `L.suchThat` (\i -> not $ S.member i used)
-          accum (S.insert ix used) ((xs !! ix):current) (j+1)
-    accum S.empty [] 0
+        ar <- newArray' n xs
+        forM [1..n] $ \i -> do
+            j <- randomRIO (i,n)
+            vi <- readArray ar i
+            vj <- readArray ar j
+            writeArray ar j vi
+            return vj
+  where
+    n = length xs
+    newArray' :: Int -> [a] -> IO (IOArray Int a)
+    newArray' n' xs' =  newListArray (1,n') xs'
+
 
 data EncContext s =
     EncContext
-        { encZero :: PaheCiph s
-        , encOne  :: PaheCiph s
+        { encZero   :: PaheCiph s
+        , encOne    :: PaheCiph s
+        , encMinOne :: PaheCiph s
         }
 
 newEncContext :: Pahe s => PahePk s -> IO (EncContext s)
@@ -53,12 +67,12 @@ newEncContext pk = do
     let k = paheK pk
     encZero <- paheEnc pk $ replicate k 0
     encOne <- paheEnc pk $ replicate k 1
+    encMinOne <- paheEnc pk $ replicate k (-1)
     pure EncContext{..}
 
--- Compute r <= c jointly. Client has r, server has c.
+-- | Compute r <= c jointly. Client has r, server has c.
 dgkClient :: Pahe s => Socket Req -> PahePk s -> EncContext s -> Int -> [Integer] -> IO (PaheCiph s)
 dgkClient sock pk EncContext{..} l rs = do
-    threadDelay 100000
 
     let k = paheK pk
     log "Client: dgk started"
@@ -69,7 +83,6 @@ dgkClient sock pk EncContext{..} l rs = do
     encRBits <- mapM (paheEnc pk) rbits
 
     cs <- mapM (paheFromBS pk) =<< receiveMulti sock
-    log "Client: dgk main body"
 
 
     log "Client: computing xors"
@@ -107,7 +120,6 @@ dgkClient sock pk EncContext{..} l rs = do
     xorsumFull3 <- paheSIMDMulScal pk (xorsums !! 0) $ replicate k 3
     cLast <- paheSIMDAdd pk deltaEnc xorsumFull3
 
-    log "Client: shuffling"
     ciShuffled <- shuffle =<< mapM (paheMultBlind pk) (cLast : ci)
 
     sendMulti sock =<< (NE.fromList <$> mapM (paheToBS pk) ciShuffled)
@@ -130,6 +142,7 @@ dgkClient sock pk EncContext{..} l rs = do
 
 dgkServer :: Pahe s => Socket Rep -> PaheSk s -> Int -> [Integer] -> IO ()
 dgkServer sock sk l cs = do
+    log "Server: dgk started"
     let pk = paheToPublic sk
     let k = paheK pk
 
@@ -137,17 +150,14 @@ dgkServer sock sk l cs = do
 --    log $ "Server cbits: " <> show cbits
 
     _ <- receive sock
-    log "Server: dgk started"
 
     sendMulti sock =<< (NE.fromList <$> mapM (paheToBS pk <=< paheEnc pk) cbits)
 
     es <- mapM (paheFromBS pk) =<< receiveMulti sock
-    log "Server: dgk computing zeroes"
     esDecr <- mapM (paheDec sk) es
     let zeroes = map (bool 1 0 . (== 0)) $
                  foldr (\e acc -> map (uncurry (*)) $ zip e acc)
                        (replicate k 1) esDecr
-    log $ "Server: zeroes " <> show zeroes
 
     enczeroes <- paheEnc pk zeroes
     send sock [] =<< paheToBS pk enczeroes
@@ -155,7 +165,7 @@ dgkServer sock sk l cs = do
     log "Server: dgk exited"
 
 
--- Compute y <= x jointly with secret inputs. Client has r, server has c.
+-- | Compute y <= x jointly with secret inputs. Client has r, server has c.
 secureCompareClient ::
        Pahe s
     => Socket Req
@@ -169,17 +179,15 @@ secureCompareClient sock pk ctx@EncContext{..} l x y = do
     log "Client: secureCompare started"
     let k = paheK pk
 
-    rhos::[Integer] <- replicateM k $ randomRIO (0, 2^(l + 80))
+    rhos::[Integer] <- replicateM k $ randomRIO (0, 2^(l + lambda) - 1)
     s0 <- paheEnc pk (map (+(2^l)) rhos)
     s1 <- paheSIMDAdd pk s0 x
     gamma <- paheSIMDSub pk s1 y
 
-    log "Client: secureCompare blinded, sent to server"
     send sock [] =<< paheToBS pk gamma
 
     cDiv2l <- paheFromBS pk =<< receive sock
 
-    log "Client: secureCompare, running dgk"
     eps <- dgkClient sock pk ctx l $ map (`mod` (2^l)) rhos
 
     epsNeg <- paheSIMDSub pk encOne eps
@@ -189,7 +197,6 @@ secureCompareClient sock pk ctx@EncContext{..} l x y = do
     delta <- paheSIMDSub pk cDiv2l rPlusEpsNeg
 
     log "Client: secureCompare exited"
-
     pure delta
 
 secureCompareServer :: Pahe s => Socket Rep -> PaheSk s -> Int -> IO ()
@@ -202,8 +209,8 @@ secureCompareServer sock sk l = do
     let cDiv2 = map (`div` (2^l)) gamma
     send sock [] =<< (paheToBS pk =<< paheEnc pk cDiv2)
 
-    log "Server: securecompare decoded blinded msg, running dgk"
     dgkServer sock sk l cMod2
+    log "Server: securecompare exited"
 
 w64ToBs :: Word64 -> ByteString
 w64ToBs = BS.pack . map fromIntegral . inbase 256 . fromIntegral
@@ -230,8 +237,8 @@ argmaxClient sock pk ctx@EncContext{..} l vals = do
             log $ "Client loop index " <> show i
             bi <- secureCompareClient sock pk ctx l
                 (vals !! (perm !! i)) curMax
-            ri <- replicateM k $ randomRIO (0, 2^(l + 80))
-            si <- replicateM k $ randomRIO (0, 2^(l + 80))
+            ri <- replicateM k $ randomRIO (0, 2^(l + lambda) - 1)
+            si <- replicateM k $ randomRIO (0, 2^(l + lambda) - 1)
             mMasked <- paheSIMDAdd pk curMax =<< paheEnc pk ri
             aMasked <- paheSIMDAdd pk (vals !! (perm !! i)) =<< paheEnc pk si
             sendMulti sock =<<
@@ -263,8 +270,8 @@ argmaxServer sock sk l m = do
     let pk = paheToPublic sk
     let k = paheK pk
 
-    let loop index i = if i == m then pure index else do
-            log $ "Server loop index " <> show i
+    let loop ixs i = if i == m then pure ixs else do
+            log $ "Server loop ixs " <> show i
             secureCompareServer sock sk l
             [bi0,mMasked,aMasked] <-
                 mapM (paheFromBS pk) =<< receiveMulti sock
@@ -280,16 +287,230 @@ argmaxServer sock sk l m = do
 
             send sock [] =<< paheToBS pk vi
 
-            let index' =
-                    map (\j -> if bi !! j == 1 then i else index !! j) [0..k-1]
+            let ixs' =
+                    map (\j -> if bi !! j == 1 then i else ixs !! j) [0..k-1]
             log "Server loop end"
-            loop index' (i+1)
+            loop ixs' (i+1)
 
-    index <- loop (replicate k 0) 1
-    log $ "Server: argmax loop ended, indices: " <> show index
+    indices <- loop (replicate k 0) 1
+    log $ "Server: argmax loop ended, indices: " <> show indices
 
     _ <- receive sock
-    sendMulti sock $ NE.fromList $ map (w64ToBs . fromIntegral) index
+    sendMulti sock $ NE.fromList $ map (w64ToBs . fromIntegral) indices
+
+    log "Server: exiting"
+
+foldCiphClient ::
+       Pahe s
+    => Socket Req
+    -> PahePk s
+    -> Int
+    -> Int -- m such that list has 2^m values
+    -> PaheCiph s
+    -> IO (PaheCiph s, PaheCiph s)
+foldCiphClient sock pk l m values = do
+    log "Client: fold start"
+    when (2^m > paheK pk) $ error $ "fold client: m is too big: " <> show (m,paheK pk)
+    when (m == 0) $ error "foldCiphClient can't fold list of 1"
+
+    let k = paheK pk
+
+    mask1 <- replicateM (2^(m-1)) $ randomRIO (0,2 ^ (l + lambda) - 1)
+    mask2 <- replicateM (2^(m-1)) $ randomRIO (0,2 ^ (l + lambda) - 1)
+    let mask3::[Integer] = mask1 <> mask2
+    mask3Enc <- paheEnc pk $ mask3 <> replicate (paheK pk - (2^m)) 0
+    valuesMasked <- paheSIMDAdd pk values mask3Enc
+
+    log "Client: masked, sent"
+    send sock [] =<< paheToBS pk valuesMasked
+
+    mask1Enc <- paheEnc pk $ map negate mask1 <> replicate (k - 2^(m-1)) 0
+    mask2Enc <- paheEnc pk $ map negate mask2 <> replicate (k - 2^(m-1)) 0
+
+    [rho1Enc,rho2Enc] <- mapM (paheFromBS pk) =<< receiveMulti sock
+    log "Client: received, unmasking"
+
+    values1 <- paheSIMDAdd pk rho1Enc mask1Enc
+    values2 <- paheSIMDAdd pk rho2Enc mask2Enc
+
+    log "Client: fold end"
+    pure (values1,values2)
+
+foldCiphServer ::
+       Pahe s
+    => Socket Rep
+    -> PaheSk s
+    -> Int -- m such that list has 2^m values
+    -> IO ()
+foldCiphServer sock sk m = do
+    let pk = paheToPublic sk
+    let k = paheK pk
+
+    rho <- (paheDec sk <=< paheFromBS pk) =<< receive sock
+    log "Server: received, splitting"
+    let (rho1,rho2) = splitAt (2^(m-1)) $ take (2^m) $ rho
+
+    rho1Enc <- paheEnc pk $ rho1 <> replicate (k - 2^(m-1)) 0
+    rho2Enc <- paheEnc pk $ rho2 <> replicate (k - 2^(m-1)) 0
+
+    log "Server: sent back"
+    sendMulti sock =<< (NE.fromList <$> mapM (paheToBS pk) [rho1Enc,rho2Enc])
+
+-- | Returns a ciphertext filled with the value of zeroth element of
+-- the input ciphertext
+fill0Client ::
+       Pahe s => Socket Req -> PahePk s -> PaheCiph s -> Int -> IO (PaheCiph s)
+fill0Client sock pk values l = do
+    maskRaw <- replicateM (paheK pk) $ randomRIO (0, 2 ^ l - 1)
+    maskEnc <- paheEnc pk maskRaw
+    valuesMasked <- paheSIMDAdd pk values maskEnc
+    send sock [] =<< paheToBS pk valuesMasked
+
+    maskEncNeg <- paheEnc pk $ map negate maskRaw
+
+    rho <- paheFromBS pk =<< receive sock
+
+    paheSIMDAdd pk rho maskEncNeg
+
+fill0Server :: Pahe s => Socket Rep -> PaheSk s -> IO ()
+fill0Server sock sk = do
+    let pk = paheToPublic sk
+    prev <- (paheDec sk <=< paheFromBS pk) =<< receive sock
+    next <- paheEnc pk $ replicate (paheK pk) (prev !! 0)
+    send sock [] =<< paheToBS pk next
+
+-- Permutes the given ciphertext with a given permutation, returns the perumt
+permuteClient ::
+       Pahe s
+    => Socket Req
+    -> PahePk s
+    -> EncContext s
+    -> Int
+    -> [Int]
+    -> PaheCiph s
+    -> IO (PaheCiph s)
+permuteClient sock pk EncContext{..} l perm values = do
+    let k = paheK pk
+    let perminv j = fromMaybe (error "permuteClient perminv") $ findIndex (==j) perm
+
+    maskRaw :: [Integer] <- replicateM k $ randomRIO (0, 2 ^ l - 1)
+    maskEnc <- paheEnc pk maskRaw
+    valuesMasked <- paheSIMDAdd pk values maskEnc
+    send sock [] =<< paheToBS pk valuesMasked
+
+    -- k ciphertexts containing valuesMasked_i in all slots
+    replElems <- mapM (paheFromBS pk) =<< receiveMulti sock
+
+    -- combine these k values into one ciphertext
+    -- loop i fills [i..k-1] values of the permuted result
+    let loop j = if j == k then pure encZero else do
+            next <- loop (j+1)
+            let i = perminv j
+            -- We select jth element from (perm^-1 j)
+            let selMask = replicate j 0 ++ [1] ++ replicate (k - j - 1) 0
+            cur <- paheSIMDMulScal pk (replElems !! i) selMask
+            paheSIMDAdd pk cur next
+
+
+    let permutedMaskNeg = map (\i -> negate (maskRaw !! (perminv i))) [0..k-1]
+
+    permuted <- loop 0
+
+    paheSIMDAdd pk permuted =<< paheEnc pk permutedMaskNeg
+
+permuteServer ::
+       Pahe s
+    => Socket Rep
+    -> PaheSk s
+    -> IO ()
+permuteServer sock sk = do
+    let pk = paheToPublic sk
+    prev <- (paheDec sk <=< paheFromBS pk) =<< receive sock
+    let dups = map (\e -> replicate (paheK pk) e) prev
+    encDups <- mapM (paheEnc pk) dups
+    sendMulti sock =<< (NE.fromList <$> mapM (paheToBS pk) encDups)
+
+
+argmaxLogClient ::
+       Pahe s
+    => Socket Req
+    -> PahePk s
+    -> EncContext s
+    -> Int
+    -> Int
+    -> PaheCiph s
+    -> IO (Int, PaheCiph s)
+argmaxLogClient sock pk ctx@EncContext{..} l m vals = do
+    let k = paheK pk
+    when (2^m > k) $ error "argmaxLogClient m is too big"
+
+    perm <- shuffle [0..k-1]
+    log $ "Client: perm " <> show perm
+    let perminv j = fromMaybe (error "argmaxLogCli perminv") $ findIndex (==j) perm
+    valsPerm <- permuteClient sock pk ctx l perm vals
+    log "Client: perm done"
+
+    let loop acc i = if i == 0 then pure acc else do
+            (p1,p2) <- foldCiphClient sock pk l i acc
+            -- delta is p2 <= p1
+            delta <- secureCompareClient sock pk ctx l p1 p2
+            -- we only care about first 2^(i-1) bits of this mask though
+            p1mask <- replicateM k $ randomRIO (0, 2 ^ l - 1)
+            p2mask <- replicateM k $ randomRIO (0, 2 ^ l - 1)
+            p1masked <- paheSIMDAdd pk p1 =<< paheEnc pk p1mask
+            p2masked <- paheSIMDAdd pk p2 =<< paheEnc pk p2mask
+            sendMulti sock =<< NE.fromList <$> mapM (paheToBS pk) [delta,p1masked,p2masked]
+
+            deltaNeg <- paheSIMDSub pk encOne delta
+
+            combinedMasked <- paheFromBS pk =<< receive sock
+            -- unmask by doing combinedMasked - delta*p1 - deltaNeg*p2
+            combined <- do
+                tmp1 <- paheSIMDMulScal pk delta (map negate p1mask)
+                tmp2 <- paheSIMDMulScal pk deltaNeg (map negate p2mask)
+                paheSIMDAdd pk combinedMasked =<< paheSIMDAdd pk tmp1 tmp2
+
+            loop combined (i-1)
+
+    maxEl <- loop valsPerm m
+
+    send sock [] ""
+    maxIndex <- fromIntegral . w64FromBs <$> receive sock
+
+    pure (perminv maxIndex, maxEl)
+
+argmaxLogServer :: Pahe s => Socket Rep -> PaheSk s -> Int -> Int -> IO ()
+argmaxLogServer sock sk l m = do
+    let pk = paheToPublic sk
+
+    permuteServer sock sk
+
+    let loop (ixs::[Integer]) i = if i == 0 then pure ixs else do
+            log $ "Server, ixs: " <> show ixs
+            log "Server starting fold"
+            foldCiphServer sock sk i
+            log "Server starting secure compare"
+            secureCompareServer sock sk l
+            [delta,p1,p2] <-
+                mapM (paheDec sk <=< paheFromBS pk) =<< receiveMulti sock
+            let pCombined = simdadd (simdmul p1 delta)
+                                    (simdmul p2 (map (\x -> 1 - x) delta))
+            send sock [] =<< paheToBS pk =<< paheEnc pk pCombined
+            -- TODO update indices
+            let ixs' =
+                    let delta' = take (2^(i-1)) delta in
+                    let (ixs0, ixs1) = splitAt (2^(i-1)) ixs in
+                    simdadd (simdmul ixs0 delta')
+                            (simdmul ixs1 (map (\x -> 1 - x) delta'))
+            loop ixs' (i-1)
+
+    ixs <- loop [0..(2^m - 1)] m
+    log $ "Server, ixs: " <> show ixs
+    let maxIx = ixs !! 0
+    log $ "Server: argmax loop ended, indices: " <> show maxIx
+
+    _ <- receive sock
+    send sock [] $ w64ToBs $ fromIntegral maxIx
 
     log "Server: exiting"
 
@@ -308,9 +529,65 @@ runProtocol =
       sk <- paheKeyGen @PailSep k
       let pk = paheToPublic sk
       eCtx <- newEncContext pk
+      let l = 7
+
+      let testLogArgmax = do
+              let m = fromIntegral $ log2 (fromIntegral k) - 1
+              vals <- replicateM (2^m) $ randomRIO (0,2^l-1)
+              putTextLn $ "m: " <> show m
+              putTextLn $ "vals: " <> show vals
+              print vals
+              let expectedMax = foldr1 max vals
+              let expectedMaxIx =
+                      fromMaybe (error "") $ findIndex (==expectedMax) vals
+              encVals <- paheEnc pk $ vals <> replicate (k - 2^m) 0
+
+              ((ix,el),()) <-
+                  measureTimeSingle "log Argmax" $
+                  concurrently
+                  (argmaxLogClient req pk eCtx l m encVals)
+                  (argmaxLogServer rep sk l m)
+
+              unless (ix == fromIntegral expectedMaxIx) $
+                  error $ "logArgmax broken, ix: " <> show (ix,expectedMaxIx)
+              decEl <- paheDec sk el
+              unless (decEl !! 0 == expectedMax) $
+                  error $ "logArgmax broken, el: " <> show (decEl !! 0, expectedMax)
+
+      let testPerm = do
+            perm <- shuffle [0..k-1]
+            putTextLn $ "perm " <> show perm
+
+            f <- replicateM k $ randomRIO (0,2^l-1)
+            print f
+            fEnc <- paheEnc pk f
+
+            (valsPerm,()) <-
+                concurrently
+                (permuteClient req pk eCtx l perm fEnc)
+                (permuteServer rep sk)
+
+            valsDec <- paheDec sk valsPerm
+            print valsDec
+
+      let testFold = do
+              let m = (fromIntegral $ log2 (fromIntegral k) - 1) - 1
+              f <- replicateM (2^m) $ randomRIO (0,2^l-1)
+              putTextLn $ "m: " <> show m
+              putTextLn $ "f: " <> show f
+              fEnc <- paheEnc pk $ f <> replicate (k-2^m) 5
+
+              ((f1,f2),()) <-
+                  measureTimeSingle "fold" $
+                  concurrently
+                  (foldCiphClient req pk l m fEnc)
+                  (foldCiphServer rep sk m)
+
+              print f
+              print =<< paheDec sk f1
+              print =<< paheDec sk f2
 
       let testArgmax = replicateM_ 1 $ do
-              let l = 64
               let m = 6
               vals <- replicateM m $ replicateM k $ randomRIO (0,2^l-1)
               print vals
@@ -318,7 +595,9 @@ runProtocol =
               encVals <- mapM (paheEnc pk) vals
 
 
-              ((maxes,indices),()) <- concurrently
+              ((maxes,indices),()) <-
+                  measureTimeSingle "Argmax" $
+                  concurrently
                   (argmaxClient req pk eCtx l encVals)
                   (argmaxServer rep sk l m)
 
@@ -330,10 +609,8 @@ runProtocol =
               if (decMaxes /= expected)
                   then error "Argmax failed" else putTextLn "OK"
 
-      testArgmax
 
       let testCompare = replicateM_ 10 $ do
-              let l = 5
               cs <- replicateM k $ randomRIO (0,2^l-1)
               rs <- replicateM k $ randomRIO (0,2^l-1)
               print cs
@@ -344,7 +621,9 @@ runProtocol =
               rsEnc <- paheEnc pk rs
 
 
-              (gamma,()) <- concurrently
+              (gamma,()) <-
+                  measureTimeSingle "SecureCompare" $
+                  concurrently
                   (secureCompareClient req pk eCtx l csEnc rsEnc)
                   (secureCompareServer rep sk l)
 
@@ -356,17 +635,19 @@ runProtocol =
                   putTextLn $ "Got:      " <> show result
                   error "Mismatch"
 
-              --putTextLn "Starting the protocol"
-              --(eps,()) <- concurrently
-              --  (dgkClient req pk l rs)
-              --  (dgkServer rep sk l cs)
+              putTextLn "Starting the protocol"
+              (eps,()) <-
+                  measureTimeSingle "DGKcomp" $
+                  concurrently
+                  (dgkClient req pk eCtx l rs)
+                  (dgkServer rep sk l cs)
 
-              --result <- map (== 1) <$> paheDec sk eps
-              --unless (result == expected) $ do
-              --    print cs
-              --    print rs
-              --    putTextLn $ "Expected: " <> show expected
-              --    putTextLn $ "Got:      " <> show result
-              --    error "Mismatch"
+              res <- map (== 1) <$> paheDec sk eps
+              unless (res == expected) $ do
+                  print cs
+                  print rs
+                  putTextLn $ "Expected: " <> show expected
+                  putTextLn $ "Got:      " <> show result
+                  error "Mismatch"
 
-      putTextLn "Protocol exited"
+      testLogArgmax
