code/experimental/rsapss/include/Hacl_Impl_Bignum_Openssl.c
@@ -3,6 +3,103 @@
 #include <openssl/bn.h>
 
 
+void Hacl_Impl_Bignum_Openssl_ossl_mod_add(
+  uint32_t nLen,
+  uint64_t *n,
+  uint64_t *a,
+  uint64_t *b,
+  uint64_t *res) {
+    BN_CTX *ctx = BN_CTX_new();
+
+    int nLenBytes = ((int)nLen)*8;
+
+    BIGNUM *bn_n = BN_lebin2bn((unsigned char*) n,nLenBytes,NULL);
+    BIGNUM *bn_a = BN_lebin2bn((unsigned char*) a,nLenBytes,NULL);
+    BIGNUM *bn_b = BN_lebin2bn((unsigned char*) b,nLenBytes,NULL);
+    BIGNUM *bn_res = BN_new ();
+
+    BN_mod_add(bn_res,bn_a,bn_b,bn_n,ctx);
+
+    if (BN_num_bytes(bn_res) > nLenBytes) {
+        printf ("nlen: %u, retlen: %u\n", nLen, BN_num_bytes(bn_res));
+        exit(1);
+    }
+
+    BN_bn2lebinpad(bn_res,(unsigned char*)res,nLenBytes);
+
+    BN_free(bn_n);
+    BN_free(bn_a);
+    BN_free(bn_b);
+    BN_free(bn_res);
+
+    BN_CTX_free(ctx);
+}
+
+void Hacl_Impl_Bignum_Openssl_ossl_mod_sub(
+  uint32_t nLen,
+  uint64_t *n,
+  uint64_t *a,
+  uint64_t *b,
+  uint64_t *res) {
+    BN_CTX *ctx = BN_CTX_new();
+
+    int nLenBytes = ((int)nLen)*8;
+
+    BIGNUM *bn_n = BN_lebin2bn((unsigned char*) n,nLenBytes,NULL);
+    BIGNUM *bn_a = BN_lebin2bn((unsigned char*) a,nLenBytes,NULL);
+    BIGNUM *bn_b = BN_lebin2bn((unsigned char*) b,nLenBytes,NULL);
+    BIGNUM *bn_res = BN_new ();
+
+    BN_mod_sub(bn_res,bn_a,bn_b,bn_n,ctx);
+
+    if (BN_num_bytes(bn_res) > nLenBytes) {
+        printf ("nlen: %u, retlen: %u\n", nLen, BN_num_bytes(bn_res));
+        exit(1);
+    }
+
+    BN_bn2lebinpad(bn_res,(unsigned char*)res,nLenBytes);
+
+    BN_free(bn_n);
+    BN_free(bn_a);
+    BN_free(bn_b);
+    BN_free(bn_res);
+
+    BN_CTX_free(ctx);
+}
+
+void Hacl_Impl_Bignum_Openssl_ossl_mod_mul(
+  uint32_t nLen,
+  uint64_t *n,
+  uint64_t *a,
+  uint64_t *b,
+  uint64_t *res) {
+    BN_CTX *ctx = BN_CTX_new();
+
+    int nLenBytes = ((int)nLen)*8;
+
+    BIGNUM *bn_n = BN_lebin2bn((unsigned char*) n,nLenBytes,NULL);
+    BIGNUM *bn_a = BN_lebin2bn((unsigned char*) a,nLenBytes,NULL);
+    BIGNUM *bn_b = BN_lebin2bn((unsigned char*) b,nLenBytes,NULL);
+    BIGNUM *bn_res = BN_new ();
+
+    BN_mod_mul(bn_res,bn_a,bn_b,bn_n,ctx);
+
+    if (BN_num_bytes(bn_res) > nLenBytes) {
+        printf ("nlen: %u, retlen: %u\n", nLen, BN_num_bytes(bn_res));
+        exit(1);
+    }
+
+    BN_bn2lebinpad(bn_res,(unsigned char*)res,nLenBytes);
+
+    BN_free(bn_n);
+    BN_free(bn_a);
+    BN_free(bn_b);
+    BN_free(bn_res);
+
+    BN_CTX_free(ctx);
+}
+
+
 void Hacl_Impl_Bignum_Openssl_ossl_mod_exp(
   uint32_t nLen,
   uint32_t expLen,
@@ -16,12 +113,9 @@ void Hacl_Impl_Bignum_Openssl_ossl_mod_exp(
     int nLenBytes = ((int)nLen)*8;
     int expLenBytes = ((int)expLen)*8;
 
-    //printf ("nLen is %u, nlenBytes is %u\n", nLen, nLenBytes);
-
     BIGNUM *bn_n = BN_lebin2bn((unsigned char*) n,nLenBytes,NULL);
     BIGNUM *bn_a = BN_lebin2bn((unsigned char*) a,nLenBytes,NULL);
     BIGNUM *bn_b = BN_lebin2bn((unsigned char*) b,expLenBytes,NULL);
-
     BIGNUM *bn_res = BN_new ();
 
     BN_mod_exp(bn_res,bn_a,bn_b,bn_n,ctx);
