code/experimental/rsapss/Hacl.Impl.Bignum.Modular.fst
@@ -21,6 +21,9 @@ open Hacl.Impl.Bignum.Addition
 open Hacl.Spec.Bignum
 
 
+val enable_ossl : bool
+let enable_ossl = true
+
 #reset-options "--z3rlimit 50 --max_fuel 0 --max_ifuel 0"
 
 val bn_remainder_core:
@@ -225,21 +228,13 @@ val bn_modular_add:
        modifies (loc res) h0 h1 /\
        as_snat h1 res = (as_snat h0 a + as_snat h0 b) % as_snat h0 n)
 let bn_modular_add #len n a b res =
-  trace "modular_add, args\n";
-  trace_lbignum n;
-  trace_lbignum a;
-  trace_lbignum b;
-  push_frame();
-  let res' = create (len +! 1ul) (uint 0) in
-  bn_add_exact a b res';
-  trace "res':\n";
-  trace_lbignum res';
-  bn_remainder res' n res;
-  trace "res:\n";
-  trace_lbignum res;
-  trace "modular_add done\n";
-  pop_frame()
-
+  if enable_ossl then ossl_mod_add #len n a b res else begin
+    push_frame();
+    let res' = create (len +! 1ul) (uint 0) in
+    bn_add_exact a b res';
+    bn_remainder res' n res;
+    pop_frame()
+  end
 
 noextract
 val sub_indifferent_zero: a:nat -> b:nat -> n:big -> Lemma
@@ -268,28 +263,29 @@ val bn_modular_sub:
        modifies (loc res) h0 h1 /\
        as_snat h1 res = (as_snat h0 a - as_snat h0 b) % as_snat h0 n)
 let rec bn_modular_sub #len n a b res =
-  if bn_is_geq a b then begin
-    push_frame();
-    let res' = create len (uint 0) in
-    let c = bn_sub a b res' in
-    assert (v c = 0);
-    bn_remainder res' n res;
-    pop_frame()
-  end else begin
-    bn_modular_sub n b a res;
-    if not (bn_is_zero res) then begin
-      bn_sub_exact n res res;
-      let h = FStar.HyperStack.ST.get () in
-      assert (as_snat h res = as_snat h n - (as_snat h b - as_snat h a) % as_snat h n);
-      to_fe_neg #(as_snat h n) (as_snat h b - as_snat h a);
-      assert (as_snat h res = (as_snat h a - as_snat h b) % as_snat h n)
+  if enable_ossl then ossl_mod_sub #len n a b res else begin
+    if bn_is_geq a b then begin
+      push_frame();
+      let res' = create len (uint 0) in
+      let c = bn_sub a b res' in
+      assert (v c = 0);
+      bn_remainder res' n res;
+      pop_frame()
     end else begin
-      let h = FStar.HyperStack.ST.get () in
-      sub_indifferent_zero (as_snat h b) (as_snat h a) (as_snat h n);
-      assert ((as_snat h a - as_snat h b) % as_snat h n = 0)
+      bn_modular_sub n b a res;
+      if not (bn_is_zero res) then begin
+        bn_sub_exact n res res;
+        let h = FStar.HyperStack.ST.get () in
+        assert (as_snat h res = as_snat h n - (as_snat h b - as_snat h a) % as_snat h n);
+        to_fe_neg #(as_snat h n) (as_snat h b - as_snat h a);
+        assert (as_snat h res = (as_snat h a - as_snat h b) % as_snat h n)
+      end else begin
+        let h = FStar.HyperStack.ST.get () in
+        sub_indifferent_zero (as_snat h b) (as_snat h a) (as_snat h n);
+        assert ((as_snat h a - as_snat h b) % as_snat h n = 0)
+      end
     end
   end
-
 
 
 val bn_modular_mul:
@@ -308,12 +304,13 @@ val bn_modular_mul:
        modifies (loc res) h0 h1 /\
        as_snat h1 res = (as_snat h0 a * as_snat h0 b) % as_snat h0 n)
 let bn_modular_mul #len n a b res =
-  push_frame ();
-  let res' = create (len +! len) (uint 0) in
-  bn_mul a b res';
-  bn_remainder res' n res;
-  pop_frame ()
-
+  if enable_ossl then ossl_mod_mul n a b res else begin
+    push_frame ();
+    let res' = create (len +! len) (uint 0) in
+    bn_mul a b res';
+    bn_remainder res' n res;
+    pop_frame ()
+  end
 
 #reset-options "--z3rlimit 200 --max_fuel 1 --max_ifuel 0 --using_facts_from '* -FStar.Seq'"
 
@@ -342,56 +339,6 @@ let bn_modular_karatsuba #nLen pow2_i n a b res =
     pop_frame ()
   end
 
-
-// // Iterative version which does not work
-//val naive_mod_exp_loop:
-//     #nLen:bn_len_strict{(v nLen + v nLen) * 64 < max_size_t}
-//  -> #expLen:bn_len_strict
-//  -> n:lbignum nLen
-//  -> a:lbignum nLen
-//  -> b:lbignum expLen
-//  -> res:lbignum nLen
-//  -> Stack unit
-//    (requires fun h ->
-//        disjoint n b /\ disjoint n res /\
-//        live h n /\ live h a /\ live h b /\ live h res /\
-//        disjoint res a /\ disjoint res b /\ disjoint n res /\
-//        as_snat h n > 1)
-//    (ensures fun h0 _ h1 -> modifies2 res b h0 h1 /\
-//        live h1 n /\ live h1 a /\ live h1 b /\ live h1 res)
-//let naive_mod_exp_loop #nLen #expLen n a b res =
-//
-//  let ctr = calc_bits b in
-//
-//  let b_is_zero = bn_is_zero b in
-//  let b_is_one = calc_bits b =. 0ul in
-//
-//  if b_is_zero then bn_assign_uint64 res (u64 1) else
-//  if b_is_one then bn_assign_bn res a else begin
-//    push_frame ();
-//
-//    let tmp1 = create nLen (uint 0) in
-//    let tmp2 = create expLen (uint 0) in
-//
-//    let one = bn_one #1ul in
-//    let y = bn_one #nLen in
-//
-//    let h0 = FStar.HyperStack.ST.get () in
-//    let inv h1 _ =
-//          modifies (loc res |+| loc b |+| loc tmp1 |+| loc tmp2 |+| loc y) h0 h1 in
-//    Lib.Loops.for 0ul ctr inv (fun i ->
-//      let odd = eq_u64 (b.(0ul) &. uint 1) (uint 1) in
-//      if not odd then begin
-//        bn_modular_mul n res res tmp1; copy res tmp1
-//      end else begin
-//        bn_modular_mul n res y tmp1; copy y tmp1;
-//        bn_modular_mul n res res tmp1; copy res tmp1
-//      end;
-//      bn_rshift1 b tmp2; copy b tmp2
-//    );
-//    bn_modular_mul n res y tmp1; copy res tmp1;
-//    pop_frame ()
-//  end
 
 val naive_mod_exp_loop:
      #nLen:bn_len_strict{(v nLen + v nLen) * 64 < max_size_t}
@@ -424,40 +371,6 @@ let rec naive_mod_exp_loop #nLen #expLen n a b res =
   end;
   pop_frame ()
 
-val bn_modular_exp_slow:
-     #nLen:bn_len_strict{v nLen * 128 < max_size_t}
-  -> #expLen:bn_len_strict
-  -> n:lbignum nLen
-  -> a:lbignum nLen
-  -> b:lbignum expLen
-  -> res:lbignum nLen
-  -> Stack unit
-    (requires fun h ->
-      live h n /\ live h a /\ live h b /\ live h res /\
-      disjoint a res /\ disjoint b res /\ disjoint n res /\
-      as_snat h n > 1)
-    (ensures  fun h0 _ h1 -> modifies1 res h0 h1 /\
-      live h1 n /\ live h1 a /\ live h1 b /\ live h1 res /\
-      (let n = as_snat h0 n in
-       as_snat h1 res = mexp (to_fe #n (as_snat h0 a)) (as_snat h0 b)))
-let bn_modular_exp_slow #nLen #expLen n a b res =
-  let h0 = FStar.HyperStack.ST.get () in
-
-  push_frame ();
-
-  memset res (uint 0) nLen;
-  res.(0ul) <- uint 1;
-  let tmp_b = create expLen (uint 0) in
-  copy tmp_b b;
-  naive_mod_exp_loop n a tmp_b res;
-
-  pop_frame ();
-
-  let h1 = FStar.HyperStack.ST.get () in
-  assume (let n' = as_snat h0 n in
-          as_snat h1 res =
-          mexp (to_fe #n' (as_snat h0 a)) (as_snat h0 b))
-
 val bn_modular_exp:
      #nLen:bn_len_strict{v nLen * 128 < max_size_t}
   -> #expLen:bn_len_strict
@@ -474,4 +387,22 @@ val bn_modular_exp:
       live h1 n /\ live h1 a /\ live h1 b /\ live h1 res /\
       (let n = as_snat h0 n in
        as_snat h1 res = mexp (to_fe #n (as_snat h0 a)) (as_snat h0 b)))
-let bn_modular_exp #nLen #expLen n a b res = ossl_mod_exp n a b res
+let bn_modular_exp #nLen #expLen n a b res =
+  if enable_ossl then ossl_mod_exp n a b res else begin
+    let h0 = FStar.HyperStack.ST.get () in
+
+    push_frame ();
+
+    memset res (uint 0) nLen;
+    res.(0ul) <- uint 1;
+    let tmp_b = create expLen (uint 0) in
+    copy tmp_b b;
+    naive_mod_exp_loop n a tmp_b res;
+
+    pop_frame ();
+
+    let h1 = FStar.HyperStack.ST.get () in
+    assume (let n' = as_snat h0 n in
+            as_snat h1 res =
+            mexp (to_fe #n' (as_snat h0 a)) (as_snat h0 b))
+  end
