code/experimental/rsapss/Hacl.Impl.Bignum.Openssl.fst
@@ -13,6 +13,55 @@ open Lib.IntTypes
 open Lib.Math.Algebra
 open Lib.Buffer
 
+
+val ossl_mod_add:
+     #len:bn_len{ (v len + 1) * 64 <= max_size_t}
+  -> n:lbignum len
+  -> a:lbignum len
+  -> b:lbignum len
+  -> res:lbignum len
+  -> Stack unit
+    (requires fun h ->
+       live h n /\ live h a /\ live h b /\ live h res /\
+       disjoint res a /\ disjoint res b /\ disjoint res n /\
+       as_snat h n > 1)
+    (ensures  fun h0 _ h1 ->
+       live h1 n /\ live h1 a /\ live h1 b /\ live h1 res /\
+       modifies (loc res) h0 h1 /\
+       as_snat h1 res = (as_snat h0 a + as_snat h0 b) % as_snat h0 n)
+
+val ossl_mod_sub:
+     #len:bn_len{ (v len + 1) * 64 <= max_size_t}
+  -> n:lbignum len
+  -> a:lbignum len
+  -> b:lbignum len
+  -> res:lbignum len
+  -> Stack unit
+    (requires fun h ->
+       live h n /\ live h a /\ live h b /\ live h res /\
+       disjoint res a /\ disjoint res b /\ disjoint res n /\
+       as_snat h n > 1)
+    (ensures  fun h0 _ h1 ->
+       live h1 n /\ live h1 a /\ live h1 b /\ live h1 res /\
+       modifies (loc res) h0 h1 /\
+       as_snat h1 res = (as_snat h0 a - as_snat h0 b) % as_snat h0 n)
+
+val ossl_mod_mul:
+     #len:bn_len_strict{v len * 128 < max_size_t}
+  -> n:lbignum len
+  -> a:lbignum len
+  -> b:lbignum len
+  -> res:lbignum len
+  -> Stack unit
+    (requires fun h ->
+       live h n /\ live h a /\ live h b /\ live h res /\
+       disjoint res a /\ disjoint res b /\ disjoint res n /\
+       as_snat h n > 1)
+    (ensures  fun h0 _ h1 ->
+       live h1 n /\ live h1 a /\ live h1 b /\ live h1 res /\
+       modifies (loc res) h0 h1 /\
+       as_snat h1 res = (as_snat h0 a * as_snat h0 b) % as_snat h0 n)
+
 val ossl_mod_exp:
      #nLen:bn_len_strict{v nLen * 128 < max_size_t}
   -> #expLen:bn_len_strict
